\documentclass[a4paper, 12pt]{article}

\usepackage[italian]{babel}

\usepackage[fleqn]{amsmath}

\begin{document}
\section*{Simulazione 2023-05-08}
Soluzione dell'integrale del punto finale del problema.

\begin{equation*}
    \begin{aligned}
        \begin{split}
            & \int_{-2}^{0} g(x) - f_1(x) dx = \\
            & \quad = \int_{-2}^{0} e^{-x} - (x^2 + 2x + 1) e^{-x} dx = \\
            & \quad = \int_{-2}^{0} (1 - x^2 - 2x - 1) e^{-x} dx = \\
            & \quad = \int_{-2}^{0} (-x^2 - 2x) e^{-x} dx = \\
            & \quad = -(\int_{-2}^{0} x^2 e^{-x} dx + \int_{-2}^{0} 2x e^{-x} dx) = \\
            & \quad = -(\left[ -x^2 e^{-x} \right]_{-2}^{0} - \int_{-2}^{0} -2x e^{-x} dx + \int_{-2}^{0} 2x e^{-x} dx) = \\
            & \quad = -(\left[ -x^2 e^{-x} \right]_{-2}^{0} + 4\int_{-2}^{0} x e^{-x} dx) = \\
            & \quad = -(\left[ -x^2 e^{-x} \right]_{-2}^{0} + 4(\left[ -x e^{-x} \right]_{-2}^{0} - \int_{-2}^{0} -e^{-x} dx)) = \\
            & \quad = -(\left[ -x^2 e^{-x} \right]_{-2}^{0} + 4(\left[ -x e^{-x} \right]_{-2}^{0} + \left[ -e^{-x} \right]_{-2}^{0})) = \\
            & \quad = -(\left[ -x^2 e^{-x} -4x e^{-x} -4e^{-x}\right]_{-2}^{0}) = \\
            & \quad = \left[ (x^2 + 4x + 4)e^{-x} \right]_{-2}^{0} = \\
            & \quad = (0^2 + 4\cdot 0 + 4)e^{0} - ((-2)^2 + 4\cdot (-2) + 4)e^{-2} = \\
            & \quad = 4 - (4 - 8 + 4)e^{-2} = \\
            & \quad = 4 - 0e^{-2} = \\
            & \quad = 4
        \end{split}
    \end{aligned}
\end{equation*}

\end{document}